1st attempt towards language equivalence

Equivalence.v
@@ -2,3 +2,164 @@ Add LoadPath "./labeled" as Labeled.
 Add LoadPath "./label-free" as LabelFree.
 Require Import Labeled.
 Require Import LabelFree.
+Require Import List.
+Require Import FSets.
+Require Import Metatheory.
+Require Import LibListSorted.
+
+Open Scope labeled_is5_scope.
+Open Scope label_free_is5_scope.
+
+Section Types.
+
+Fixpoint labeled_type (A: ty_LF) : ty_L :=
+match A with
+| tvar_LF => tvar_L
+| tarrow_LF A' A'' => tarrow_L (labeled_type A') (labeled_type A'')
+| tbox_LF A' => tbox_L (labeled_type A')
+| tdia_LF A' => tdia_L (labeled_type A')
+end.
+
+Fixpoint label_free_type (A: ty_L) : ty_LF :=
+match A with
+| tvar_L => tvar_LF
+| tarrow_L A' A'' => tarrow_LF (label_free_type A') (label_free_type A'')
+| tbox_L A' => tbox_LF (label_free_type A')
+| tdia_L A' => tdia_LF (label_free_type A')
+end.
+
+Lemma types_id1:
+forall A: ty_L,
+  labeled_type ( label_free_type A )  = A.
+intros;
+induction A; simpl.
+  reflexivity.
+  rewrite IHA1; rewrite IHA2; reflexivity.
+  rewrite IHA; reflexivity.
+  rewrite IHA; reflexivity.
+Qed.
+
+Lemma types_id2:
+forall A: ty_LF,
+  label_free_type ( labeled_type A )  = A.
+intros;
+induction A; simpl.
+  reflexivity.
+  rewrite IHA1; rewrite IHA2; reflexivity.
+  rewrite IHA; reflexivity.
+  rewrite IHA; reflexivity.
+Qed.
+
+End Types.
+
+Section Contexts.
+
+(* Labeled from label-free *)
+
+Fixpoint give_names (G: list Context_LF) (Used: worlds_L) :=
+match G with
+| nil => nil
+| Gamma::G' => 
+  let w := var_gen Used in
+    (Gamma, w) :: give_names G' (\{w} \u Used)
+end.
+
+Fixpoint find_fst_eq (L:list (Context_LF * var)) (el: Context_LF) :=
+match L with
+| nil => error
+| (G, w) :: L' => If G = el then Some w else find_fst_eq L' el
+end.
+
+Definition annotate_worlds (p: (Context_LF * var)) :=
+match p with
+| (L, w) => map (fun (x: ty_LF) => (labeled_type x, fwo w)) L
+end.
+
+Definition labeled_context (G: Background_LF) (Gamma: Context_LF) : option (worlds_L * Context_L * var) :=
+  let CtxLst := give_names (Gamma::G) \{} in
+  let w := find_fst_eq CtxLst Gamma in
+  let Omega := from_list (map snd CtxLst) in
+  let Delta := flat_map annotate_worlds CtxLst in
+  match w with
+    | error => error (* this is never going to happen! *)
+    | Some w' => Some (Omega, Delta, w')
+  end.
+
+
+(* Label-free from labeled *)
+
+Fixpoint find_and_append (a: ty_L) (w:var) (res: list (list ty_LF * var)) :=
+match res with
+| nil => (((label_free_type a)::nil), w) :: nil
+| (Gamma, w') :: res' => 
+  If w = w' then ((label_free_type a)::Gamma, w') :: res' else find_and_append a w res'
+end.
+  
+Fixpoint find_snd_eq (L:list (Context_LF * var)) (el: var) :=
+match L with
+| nil => error
+| (G, w) :: L' => If w = el then Some G else find_snd_eq L' el
+end.
+
+Theorem eq_pair_ty_w_dec:
+forall a b: list ty_LF * var, {a = b} + {a <> b}.
+intros;
+decide equality.
+apply eq_var_dec.
+decide equality.
+decide equality.
+Qed.
+
+(* TODO: Result? really? *)
+Fixpoint group_contexts (Omega: worlds_L) (Forgotten: worlds_L) (Gamma: Context_L) (Result : list (Context_LF * var)) :=
+match Gamma with
+| nil => (map (fun (x:Context_LF * var) => (rev (fst x), snd x)) Result) 
+   (* should be:
+      ++ generate_empty (cardinal Omega)  
+      for now we will ignore fresh, unused worlds *)
+| (a, fwo w)::Gamma' => let Result' := find_and_append a w Result in
+    group_contexts (Omega \- \{w}) (\{w} \u Forgotten) Gamma' Result'
+| _ :: Gamma' => (* we need to get rid of this case! *) group_contexts Omega Forgotten Gamma' Result
+end.
+
+Definition label_free_context (Omega: worlds_L) (Gamma: Context_L) (w: var) : option(Background_LF * Context_LF) :=
+ let contexts := group_contexts Omega \{} Gamma nil in
+ let Gamma' := find_snd_eq contexts w in
+ match Gamma' with
+ | error => error
+ | Some Gamma'' => 
+    let G := map fst (remove eq_pair_ty_w_dec (Gamma'', w) contexts) in
+      Some (G, Gamma'')  
+ end. 
+
+Lemma labeled_context_no_error:
+forall G Gamma,
+  labeled_context G Gamma <> error.
+Admitted.
+
+Lemma label_free_context_no_error:
+forall Omega Gamma w,
+  label_free_context Omega Gamma w <> error.
+Admitted.
+
+Lemma contexts_equiv1:
+forall G Gamma Omega Delta w G' Gamma'
+  (HT1: labeled_context G Gamma = Some (Omega, Delta, w))
+  (HT2: label_free_context Omega Delta w = Some (G', Gamma')),
+    permut G G' /\
+    Gamma = Gamma'.
+Admitted.
+
+Lemma contexts_equiv2:
+forall Omega Gamma w G Delta Omega' Gamma' w'
+  (HT1: label_free_context Omega Gamma w = Some (G, Delta))
+  (HT2: labeled_context G Delta = Some (Omega', Gamma', w')),
+    (forall X, X \in Omega  <-> X \in Omega') /\
+    Gamma = Gamma' /\
+    w = w'.
+Admitted.
+
+End Contexts.
+
+Close Scope labeled_is5_scope.
+Close Scope label_free_is5_scope.
